feat: Add helper functions around bytes (#960)

Veir/Data/LLVM/Byte/Basic.lean
@@ -5,8 +5,6 @@ public import Veir.Data.LLVM.Int.Bitblast
 
 namespace Veir.Data.LLVM
 
-namespace Byte
-
 public section
 
 /--
@@ -22,6 +20,18 @@ structure Byte (w : Nat) where
   /-- Invariant: if a bit is poison, the corresponding bit in `val` is zero. -/
   h : val &&& poison = 0
 deriving DecidableEq
+
+namespace Byte
+
+def cast {w₁ w₂ : Nat} (x : Byte w₁) (h : w₁ = w₂) : Byte w₂ :=
+  ⟨x.val.cast h, x.poison.cast h, by simp [x.h]⟩
+
+@[simp, grind =]
+theorem cast_self {w : Nat} (x : Byte w) (h : w = w) : cast x h = x := by
+  simp [cast]
+
+def allPoison : Byte w :=
+  ⟨0, BitVec.allOnes w, by simp⟩
 
 def and (x y : Byte w) : Byte w :=
   let poison := x.poison ||| y.poison
@@ -41,13 +51,35 @@ def xor (x y : Byte w) : Byte w :=
 
 instance {w : Nat} : XorOp (Byte w) := ⟨xor⟩
 
+def trunc (x : Byte w) (w' : Nat) : Byte w' :=
+  ⟨x.val.truncate w', x.poison.truncate w', by (
+    simp [←BitVec.setWidth_and, x.h]
+  )⟩
+
+def lshr (x : Byte w) (y : Int w) : Byte w := Id.run do
+  let .val y := y | allPoison
+
+  if y ≥ w then
+    return allPoison
+
+  ⟨x.val >>> y, x.poison >>> y, by (
+    simp [←BitVec.ushiftRight_and_distrib, x.h]
+  )⟩
+
+def toString_rec {w : Nat} (b : Byte w) : String :=
+  if w = 0 then "" else
+  s!"{if b.poison.getMsbD 0 then "?" else ToString.toString (b.val.getMsbD 0).toNat}{(b.trunc (w - 1)).toString_rec}"
+
+instance {w : Nat} : ToString (Byte w) where
+  toString (b : Byte w) := s!"0b{b.toString_rec}#{w}"
+
 open Int
 
 /-- Convert from `Byte` and `Int`.
   A byte where no bit is poison is equal to an integer value.
   If any bit is poison, the integer type is also poison.
 -/
-def Byte.toInt {w : Nat} (x : Byte w) : Int w :=
+def toInt {w : Nat} (x : Byte w) : Int w :=
   if x.poison = 0 then
     .val x.val
   else
@@ -58,6 +90,33 @@ def fromInt {w : Nat} (x : Int w) : Byte w :=
     ⟨0, BitVec.allOnes w, by simp⟩
   else
     ⟨x.getValue, 0, by simp⟩
-end
+
+def toUInt64 (x : Byte 64) : UInt64 :=
+  if x.poison = 0 then
+    UInt64.ofBitVec x.val
+  else
+    0
+
+def fromUInt64 (x : UInt64) : Byte 64 :=
+  ⟨x.toBitVec, 0, by simp⟩
+
+/--
+  i is refined by i' if for each bit, either i is poison, or the bits are the same and i' is not poison.
+-/
+@[simp, grind .]
+def isRefinedBy {w : Nat} (i i' : Veir.Data.LLVM.Byte w) : Prop :=
+  (i.poison ||| ((i.val ^^^ ~~~i'.val) &&& ~~~i'.poison)) = BitVec.allOnes w
+
+@[inherit_doc] infix:50 " ⊒ " => LLVM.Byte.isRefinedBy
+
+@[simp, grind .]
+theorem isRefinedBy_refl {w : Nat} (i : Byte w) : i ⊒ i := by
+  grind
+
+theorem isRefinedBy_trans {w : Nat} {i j k : Byte w}
+    (h₁ : i ⊒ j) (h₂ : j ⊒ k) : i ⊒ k := by
+  grind
 
 end Byte
+
+end
